theories/Hole.v
@@ -1,44 +1,121 @@
 From LambdaST Require Import
+  FV
+  Ident
   Context.
+
+From Hammer Require Import Tactics.
 
 Inductive hole : Set :=
   | HoleHere
-  | HoleCommaL (lhs : hole) (rhs : context)
-  | HoleCommaR (lhs : context) (rhs : hole)
-  | HoleSemicL (lhs : hole) (rhs : context)
-  | HoleSemicR (lhs : context) (rhs : hole)
+  | HoleCommaL (h : hole) (g : context)
+  | HoleCommaR (g : context) (h : hole)
+  | HoleSemicL (h : hole) (g : context)
+  | HoleSemicR (g : context) (h : hole)
   .
 
-Fixpoint fill h y :=
+Fixpoint fill h D :=
   match h with
-  | HoleHere => y
-  | HoleCommaL lhs rhs => CtxComma (fill lhs y) rhs
-  | HoleCommaR lhs rhs => CtxComma lhs (fill rhs y)
-  | HoleSemicL lhs rhs => CtxSemic (fill lhs y) rhs
-  | HoleSemicR lhs rhs => CtxSemic lhs (fill rhs y)
+  | HoleHere => D
+  | HoleCommaL lhs rhs => CtxComma (fill lhs D) rhs
+  | HoleCommaR lhs rhs => CtxComma lhs (fill rhs D)
+  | HoleSemicL lhs rhs => CtxSemic (fill lhs D) rhs
+  | HoleSemicR lhs rhs => CtxSemic lhs (fill rhs D)
   end.
 
-Inductive FillWith y : hole -> context -> Prop :=
+Inductive FillWith d : hole -> context -> Prop :=
   | FillHere :
-      FillWith y HoleHere y
-  | FillCommaL : forall lhs rhs lhs',
-      FillWith y lhs lhs' ->
-      FillWith y (HoleCommaL lhs rhs) (CtxComma lhs' rhs)
-  | FillCommaR : forall lhs rhs rhs',
-      FillWith y rhs rhs' ->
-      FillWith y (HoleCommaR lhs rhs) (CtxComma lhs rhs')
-  | FillSemicL : forall lhs rhs lhs',
-      FillWith y lhs lhs' ->
-      FillWith y (HoleSemicL lhs rhs) (CtxSemic lhs' rhs)
-  | FillSemicR : forall lhs rhs rhs',
-      FillWith y rhs rhs' ->
-      FillWith y (HoleSemicR lhs rhs) (CtxSemic lhs rhs')
+      FillWith d HoleHere d
+  | FillCommaL : forall h g' g,
+      FillWith d h g ->
+      FillWith d (HoleCommaL h g') (CtxComma g g')
+  | FillCommaR : forall g h g',
+      FillWith d h g' ->
+      FillWith d (HoleCommaR g h) (CtxComma g g')
+  | FillSemicL : forall h g' g,
+      FillWith d h g ->
+      FillWith d (HoleSemicL h g') (CtxSemic g g')
+  | FillSemicR : forall g h g',
+      FillWith d h g' ->
+      FillWith d (HoleSemicR g h) (CtxSemic g g')
   .
 
-Theorem reflect_fill : forall h y c,
-  c = fill h y <-> FillWith y h c.
+Theorem reflect_fill : forall h d g,
+  g = fill h d <-> FillWith d h g.
 Proof.
   split; intros.
-  - subst. generalize dependent y. induction h; intros; simpl in *; constructor; apply IHh.
+  - subst. generalize dependent d. induction h; intros; simpl in *; constructor; apply IHh.
   - induction H; simpl; try rewrite IHFillWith; reflexivity.
+Qed.
+
+
+Fixpoint hole_fv (h : hole) : set ident :=
+  match h with
+  | HoleHere => FV.empty
+  | HoleCommaL h g
+  | HoleCommaR g h
+  | HoleSemicL h g
+  | HoleSemicR g h => FV.union (hole_fv h) (fv g)
+  end.
+
+Instance hole_fv_inst : FV hole :=
+{
+  fv := hole_fv
+}.
+
+Theorem fill_fv_reflect: forall H D G,
+  FillWith H D G ->
+  forall x, fv G x <-> fv H x \/ fv D x.
+Proof.
+  intros H D G Hfill.
+  induction Hfill; sfirstorder.
+Qed.
+
+
+Theorem fill_fv : forall H D,
+  forall x, fv (fill H D) x <-> fv H x \/ fv D x.
+Proof.
+  intros H D.
+  remember (fill H D).
+  hauto lq: on use:fill_fv_reflect, reflect_fill.
+Qed.
+
+Inductive wf_hole : hole -> Prop :=
+| wf_HoleHere : wf_hole HoleHere
+| wf_HoleCommaL : forall h g,
+  wf_hole h ->
+  wf_ctx g ->
+  disjoint (fv h) (fv g) ->
+  wf_hole (HoleCommaL h g)
+| wf_HoleCommaR : forall h g,
+  wf_hole h ->
+  wf_ctx g ->
+  disjoint (fv h) (fv g) ->
+  wf_hole (HoleCommaR g h)
+| wf_HoleSemicL : forall h g,
+  wf_hole h ->
+  wf_ctx g ->
+  disjoint (fv h) (fv g) ->
+  wf_hole (HoleSemicL h g)
+| wf_HoleSemicR : forall h g,
+  wf_hole h ->
+  wf_ctx g ->
+  disjoint (fv h) (fv g) ->
+  wf_hole (HoleSemicR g h)
+.
+
+Theorem wf_fill_reflect : forall h d g,
+  FillWith d h g ->
+  wf_ctx g ->
+  wf_hole h /\ wf_ctx d /\ disjoint (fv h) (fv d).
+Proof.
+  intros h d g H. induction H; cbn in *; intros; sauto lq: on use:fill_fv_reflect.
+Qed.
+
+Theorem wf_fill : forall h d,
+  wf_ctx (fill h d) -> (wf_hole h /\ wf_ctx d /\ disjoint (fv h) (fv d)).
+Proof.
+  intros h d.
+  remember (fill h d) as g.
+  apply reflect_fill in Heqg.
+  best use: wf_fill_reflect.
 Qed.
