theories/FV.v
@@ -1,0 +1,24 @@
+From LambdaST Require Import
+  Ident.
+
+Definition set A := A -> Prop.
+
+Definition empty {A : Type} : set A := fun _ => False.
+
+Definition singleton {A : Type} (x : A) : set A :=
+    fun y => x = y.
+
+Definition union {A : Type} (X Y : set A) : set A :=
+    fun x => X x \/ Y x.
+
+Definition intersection {A : Type} (X Y : set A) : set A :=
+    fun x => X x /\ Y x.
+
+Definition minus {A : Type} (X Y : set A) : set A :=
+    fun x => X x /\ ~(Y x).
+
+Definition disjoint {A : Type} (X Y : set A) : Prop :=
+    (forall x, X x -> ~(Y x)) /\ (forall x, Y x -> ~(X x)).
+
+Class FV (A : Type) :=
+  { fv : A -> set ident }.
