theories/SemSound.v
@@ -3,7 +3,8 @@ From LambdaST Require Import
     Semantics
     Typing
     Prefix
-    Environment.
+    Environment
+    Context.
 Require Import Coq.Program.Equality.
 
 From Hammer Require Import Tactics.
@@ -11,9 +12,29 @@ From Hammer Require Import Tactics.
 
 Theorem soundout : forall G e e' s eta p,
     Typed G e s ->
-    EnvTyped eta G ->
     Step eta e e' p ->
+    wf e ->
+    wf_ctx G ->
+    EnvTyped eta G ->
     PfxTyped p s
 .
 Proof.
+    intros G e e' s eta p Hty.
+    generalize dependent e'.
+    generalize dependent eta.
+    generalize dependent p.
+    induction Hty; intros p eta e0' Hstep Hwfe HwfG Heta.
+    - sauto lq: on rew: off.
+    - sinvert Hwfe; sinvert Hstep; eapply IHHty.
+      + eauto.
+      + eauto.
+      + admit.
+      + admit.
+    - sinvert Hwfe. admit.
+    - sinvert Hwfe. admit.
+    - sinvert Hwfe. admit.
+    - sinvert Hwfe. admit.
+    - sinvert Hwfe. admit.
+    - admit.
+    - admit.
 Admitted.
