theories/Typing.v
@@ -2,6 +2,7 @@ From LambdaST Require Import
   Context
   Terms
   Types
+  FV
   Hole.
 From Coq Require Import
   List.
@@ -34,7 +35,7 @@ Inductive Typed : context -> term -> type -> Prop :=
   | T_Var : forall G x s,
       fill G (CtxHasTy x s) |- (TmVar x) \in s
   | T_SubCtx : forall G G' e s,
-      (* Contains G' G -> *)
+      sub_ctx G G' ->
       G' |- e \in s ->
       G |- e \in s
   | T_Let : forall G D x e e' s t,
@@ -45,5 +46,10 @@ where "G '|-' x '\in' T" := (Typed G x T).
 
 Theorem typing_fv : forall G e s,
     G |- e \in s ->
-    forall x, In x (fv e) -> In x (vars_in G).
+    forall x, fv e x -> fv G x.
+Proof.
+    intros G e s H.
+    induction H; intros x0 Hfv.
+    - sfirstorder.
+    - sfirstorder.
 Admitted.
